artifact tests

test/artifact/pneutube/crypto/Hacl.Test.fst
@@ -162,6 +162,68 @@ let test_curve25519 () =
   TestLib.compare_and_print curve25519 expected2 result keysize;
   pop_frame()
 
+val test_box: unit -> Stack unit
+  (requires (fun h -> True))
+  (ensures  (fun h0 r h1 -> True))
+let test_box () =
+  push_frame();
+  (* Sizes *)
+  let len = 47ul in
+  let len_64 = 47uL in
+  let keysize = 32ul in
+  let noncesize = 24ul in
+  let macsize = 16ul in
+  (* Storage buffers *)
+  let pk1 = create 0uy keysize in
+  let pk2 = create 0uy keysize in
+  let nm1 = create 0uy keysize in
+  let nm2 = create 0uy keysize in
+  let ciphertext = create 0uy (FStar.UInt32 (len +^ 16ul)) in
+  let mac = create 0uy macsize in
+  let plaintext = create 0uy len in
+  let result    = create 0uy len in
+  let nonce = createL [
+    0x00uy; 0x01uy; 0x02uy; 0x03uy;
+    0x04uy; 0x05uy; 0x06uy; 0x07uy;
+    0x08uy; 0x09uy; 0x10uy; 0x11uy;
+    0x12uy; 0x13uy; 0x14uy; 0x15uy;
+    0x16uy; 0x17uy; 0x18uy; 0x19uy;
+    0x20uy; 0x21uy; 0x22uy; 0x23uy
+    ] in
+  let sk1 = createL [
+    0x00uy; 0x01uy; 0x02uy; 0x03uy;
+    0x04uy; 0x05uy; 0x06uy; 0x07uy;
+    0x08uy; 0x09uy; 0x10uy; 0x11uy;
+    0x12uy; 0x13uy; 0x14uy; 0x15uy;
+    0x16uy; 0x17uy; 0x18uy; 0x19uy;
+    0x20uy; 0x21uy; 0x22uy; 0x23uy;
+    0x24uy; 0x25uy; 0x26uy; 0x27uy;
+    0x28uy; 0x29uy; 0x30uy; 0x31uy
+    ] in
+  let sk2 = createL [
+    0x31uy; 0x30uy; 0x29uy; 0x28uy;
+    0x27uy; 0x26uy; 0x25uy; 0x24uy;
+    0x23uy; 0x22uy; 0x21uy; 0x20uy;
+    0x19uy; 0x18uy; 0x17uy; 0x16uy;
+    0x15uy; 0x14uy; 0x13uy; 0x12uy;
+    0x11uy; 0x10uy; 0x09uy; 0x08uy;
+    0x07uy; 0x06uy; 0x05uy; 0x04uy;
+    0x03uy; 0x02uy; 0x01uy; 0x00uy
+    ] in
+  let basepoint = create 0uy 32ul in
+  basepoint.(0ul) <- 9uy;
+  Hacl.EC.Curve25519.exp pk1 basepoint sk1;
+  Hacl.EC.Curve25519.exp pk2 basepoint sk2;
+  let _ = Hacl.Box.crypto_box_easy ciphertext plaintext len_64 nonce pk1 sk2 in
+  let _ = Hacl.Box.crypto_box_open_easy result ciphertext (FStar.UInt64 (len_64 +^ 16uL)) nonce pk2 sk1 in
+  let str_encr2 = createL [
+    0x53y; 0x6fy; 0x64y; 0x69y; 0x75y; 0x6dy; 0x27y; 0x73y;
+    0x20y; 0x42y; 0x6fy; 0x78y; 0x2fy; 0x55y; 0x6ey; 0x62y;
+    0x6fy; 0x78y; 0y
+  ] (* Buffer literal for 'Sodium's Box/Unbox' *) in
+  TestLib.compare_and_print str_encr2 plaintext result len;
+  pop_frame()
+
 val main: unit -> ST FStar.Int32.t
   (requires (fun h -> True))
   (ensures  (fun h0 r h1 -> True))
@@ -169,4 +231,5 @@ let main () =
   test_poly1305_64 ();
   test_xsalsa20 ();
   test_curve25519 ();
+  test_box ();
   C.exit_success
